src/Mail2/MailServerLockAbsImpl.v
@@ -3,21 +3,15 @@ Require Import String.
 Require Import MailServerAPI.
 Require Import MailServerLockAbsAPI.
 
+Module MailServerLockAbsImpl' <:
+  LayerImplAbsT MailServerOp
+    MailServerLockAbsState MailServerLockAbsAPI
+    MailServerState MailServerAPI.
 
-Module MailServerLockAbsImpl <: LayerImpl MailServerLockAbsAPI MailServerAPI.
+  Import MailServerLockAbsState.
 
-  Definition absR (s1 : MailServerLockAbsAPI.State) (s2 : MailServerAPI.State) :=
-    MailServerLockAbsAPI.maildir s1 = s2.
-
-  Definition compile_ts (ts : @threads_state MailServerAPI.opT) := ts.
-
-  Theorem compile_ts_no_atomics :
-    forall (ts : @threads_state MailServerAPI.opT),
-      no_atomics_ts ts ->
-      no_atomics_ts (compile_ts ts).
-  Proof.
-    unfold compile_ts; eauto.
-  Qed.
+  Definition absR (s1 : MailServerLockAbsState.State) (s2 : MailServerState.State) :=
+    MailServerLockAbsState.maildir s1 = s2.
 
   Hint Extern 1 (MailServerAPI.step _ _ _ _ _ _) => econstructor.
 
@@ -30,29 +24,20 @@ Module MailServerLockAbsImpl <: LayerImpl MailServerLockAbsAPI MailServerAPI.
     all: eauto.
   Qed.
 
-  Hint Resolve absR_ok.
-
-  Theorem compile_traces_match :
-    forall ts,
-      no_atomics_ts ts ->
-      traces_match_abs absR
-        MailServerLockAbsAPI.initP
-        MailServerLockAbsAPI.step
-        MailServerAPI.step (compile_ts ts) ts.
-  Proof.
-    unfold compile_ts, traces_match_abs; intros.
-    eexists; intuition idtac.
-    eapply trace_incl_abs; eauto.
-    eauto.
-  Qed.
-
   Theorem absInitP :
     forall s1 s2,
-      MailServerLockAbsAPI.initP s1 ->
+      MailServerLockAbsState.initP s1 ->
       absR s1 s2 ->
-      MailServerAPI.initP s2.
+      MailServerAPI.MailServerState.initP s2.
   Proof.
     eauto.
   Qed.
 
-End MailServerLockAbsImpl.
+End MailServerLockAbsImpl'.
+
+Module MailServerLockAbsImpl :=
+  LayerImplAbs MailServerOp
+    MailServerLockAbsState MailServerLockAbsAPI
+    MailServerState MailServerAPI
+    MailServerLockAbsImpl'.
+    
